tcfg/Tagle.v
@@ -2,12 +2,13 @@ Require Import Program.Equality.
 Require Export ListExtra PreSuffix ListOrder.
 
 Definition Tag := list nat.
+
+(** * Tagle: relation that relates tags lexically *)
   
 Inductive Tagle : Tag -> Tag -> Prop :=
 | TgApp (i : Tag) : Tagle nil i
 | TgEq  (n : nat) (i j : Tag) : Tagle i j -> Tagle (i :r: n) (j :r: n)
 | TgLt (n m : nat) (i j : Tag) : n < m -> Tagle (i :r: n) (j :r: m).
-
 
 Infix "⊴" := Tagle (at level 70).
 
@@ -28,7 +29,6 @@ Proof.
   - rewrite <-cons_rcons_assoc. econstructor;eauto.
   - rewrite <-cons_rcons_assoc. econstructor;eauto.
 Qed.
-
 
 Lemma Tagle_refl (i : Tag)
   : i ⊴ i.
@@ -91,141 +91,71 @@ Proof.
         -- econstructor;auto. omega.
         -- subst. econstructor. auto.
 Qed.
-
-  (** tagging order **)
-
-  Fixpoint tagle' (i j : Tag)
-    := match i,j with
-       | nil,_ => True
-       | _ :: _, nil => False
-       | n :: i, m :: j => if decision (n < m)
-                        then True
-                        else if decision (n = m)
-                             then tagle' i j
-                             else False
-       end.
   
-  Global Instance Tagle_PartialOrder : PartialOrder eq Tagle.
-  Proof.
-    econstructor;intros.
-    - subst. econstructor;unfold Basics.flip; eapply Tagle_refl.
-    - inversion H. unfold Basics.flip in H1. clear H.
-      revert dependent H1.
-      induction H0;intros.
-      + inversion H1;try congruence'. reflexivity.
-      + inversion H1;[congruence' | |].
-        * f_equal. eapply rcons_eq1 in H. eapply rcons_eq1 in H2.
-          subst. eauto.
-        * exfalso. eapply rcons_eq2 in H. eapply rcons_eq2 in H2. subst. omega.
-      + inversion H1;[congruence' | |].
-        * exfalso. eapply rcons_eq2 in H0. eapply rcons_eq2 in H2. subst. omega.
-        * exfalso. eapply rcons_eq2 in H0. eapply rcons_eq2 in H2. subst. omega.
-  Qed.
-
-  
-
-  Lemma prefix_tagle (i j : Tag)
-        (Hpre : Prefix i j)
-    : i ⊴ j.
-  Proof.
-    induction Hpre;
-      eauto with tagle.
-  Qed.
-
-  Lemma Tagle_app2 (i j k : Tag)
-        (H : i ++ k ⊴ j ++ k)
-    : i ⊴ j.
-  Proof.
-    rinduction k.
-    - do 2 rewrite app_nil_r in H. assumption.
-    - eapply H.
-      inversion H0.
-      + destruct l;cbn in H2;congruence'.
-      + rewrite app_rcons_assoc in H1. eapply rcons_eq1 in H1.
-        rewrite app_rcons_assoc in H2. eapply rcons_eq1 in H2.
+Global Instance Tagle_PartialOrder : PartialOrder eq Tagle.
+Proof.
+  econstructor;intros.
+  - subst. econstructor;unfold Basics.flip; eapply Tagle_refl.
+  - inversion H. unfold Basics.flip in H1. clear H.
+    revert dependent H1.
+    induction H0;intros.
+    + inversion H1;try congruence'. reflexivity.
+    + inversion H1;[congruence' | |].
+      * f_equal. eapply rcons_eq1 in H. eapply rcons_eq1 in H2.
         subst. eauto.
-      + rewrite app_rcons_assoc in H1. eapply rcons_eq2 in H1.
-        rewrite app_rcons_assoc in H2. eapply rcons_eq2 in H2.
-        subst. omega.
-  Qed.
-  
-  Lemma Tagle_cons2 (i : Tag) (n m : nat)
-        (Hle : n <= m)
-    : n :: i ⊴ m :: i.
-  Proof.
-    rinduction i.
-    - fold (nil ++ [n]). fold ([] ++ [m]).
-      fold ([] :r: n). fold ([] :r: m).
-      eapply le_lt_or_eq in Hle.
-      destruct Hle;subst;econstructor;eauto.
-      reflexivity.
-    - do 2 rewrite <-cons_rcons_assoc. econstructor;eauto.
-  Qed.
+      * exfalso. eapply rcons_eq2 in H. eapply rcons_eq2 in H2. subst. omega.
+    + inversion H1;[congruence' | |].
+      * exfalso. eapply rcons_eq2 in H0. eapply rcons_eq2 in H2. subst. omega.
+      * exfalso. eapply rcons_eq2 in H0. eapply rcons_eq2 in H2. subst. omega.
+Qed.
 
-  Lemma tagle_prefix_hd_le (n m : nat) (i j : Tag)
-        (H2 : m :: i ⊴ j)
-        (H1 : Prefix (n :: i) j)
-    : m <= n.
-  Proof.
-    eapply prefix_eq in H1.
-    destructH.
-    subst. rewrite app_cons_assoc in H2. fold ([m] ++ i) in H2. eapply Tagle_app2 in H2.
-    fold (nil ++ [m]) in H2.
-    fold ([] :r: m) in H2.
-    eapply Tagle_le;eauto.
-  Qed.
-  
-(*      
-      
+Lemma prefix_tagle (i j : Tag)
+      (Hpre : Prefix i j)
+  : i ⊴ j.
+Proof.
+  induction Hpre;
+    eauto with tagle.
+Qed.
 
-  (* the tags have to be reversed bc. the head is least significant *)
-  Definition tagle (i j : Tag) := tagle' (rev i) (rev j).
+Lemma Tagle_app2 (i j k : Tag)
+      (H : i ++ k ⊴ j ++ k)
+  : i ⊴ j.
+Proof.
+  rinduction k.
+  - do 2 rewrite app_nil_r in H. assumption.
+  - eapply H.
+    inversion H0.
+    + destruct l;cbn in H2;congruence'.
+    + rewrite app_rcons_assoc in H1. eapply rcons_eq1 in H1.
+      rewrite app_rcons_assoc in H2. eapply rcons_eq1 in H2.
+      subst. eauto.
+    + rewrite app_rcons_assoc in H1. eapply rcons_eq2 in H1.
+      rewrite app_rcons_assoc in H2. eapply rcons_eq2 in H2.
+      subst. omega.
+Qed.
 
+Lemma Tagle_cons2 (i : Tag) (n m : nat)
+      (Hle : n <= m)
+  : n :: i ⊴ m :: i.
+Proof.
+  rinduction i.
+  - fold (nil ++ [n]). fold ([] ++ [m]).
+    fold ([] :r: n). fold ([] :r: m).
+    eapply le_lt_or_eq in Hle.
+    destruct Hle;subst;econstructor;eauto.
+    reflexivity.
+  - do 2 rewrite <-cons_rcons_assoc. econstructor;eauto.
+Qed.
 
-  Global Instance tagle'_PreOrder : PreOrder tagle'.
-  econstructor.
-  - unfold Reflexive. intros x. induction x;cbn;auto.
-    decide (a < a);[omega|].
-    decide (a = a);[auto|omega].
-  - intros x. induction x; intros y z Hxy Hyz;cbn in *;auto.
-    destruct y;[contradiction|];cbn in *.
-    destruct z;[contradiction|];cbn in *.
-    decide (a < n0);[auto|].
-    decide (a < n); decide (n < n0).
-    + exfalso. omega.
-    + exfalso. assert (n0 < n) by omega. decide (n = n0);[omega|contradiction].
-    + exfalso. assert (n < a) by omega. decide (a = n);[omega|contradiction].
-    + decide (a = n); decide (n = n0). 2-4: contradiction.
-      subst a. decide (n = n0);[|contradiction].
-      eapply IHx;eauto.
-  Qed.
-
-  Global Instance tagle'_PartialOrder : PartialOrder eq tagle'.
-  econstructor;intros.
-  - subst. econstructor. 2: unfold Basics.flip. all: eapply tagle'_PreOrder.
-  - inversion H. clear H. unfold Basics.flip in H1.
-    revert dependent x. induction x0;intros;cbn in *.
-    + destruct x; cbn in *;[auto|contradiction].
-    + destruct x; cbn in *;[contradiction|].
-      decide (n = a).
-      * decide (a = n);[|omega]. decide (n < a); decide (a < n). 1-3:omega. subst.
-        f_equal. eapply IHx0;eauto.
-      * decide (n < a);[|contradiction].
-        decide (a < n);[omega|].
-        decide (a = n);[omega|contradiction].
-  Qed.
-
-  Global Instance tagle_Preorder : PreOrder tagle.
-  econstructor.
-  - unfold Reflexive. intros x. unfold tagle. eapply tagle'_PreOrder.
-  - unfold Transitive, tagle. intros. eapply tagle'_PreOrder;eauto.
-  Qed.
-
-  Global Instance tagle_PartialOrder : PartialOrder eq tagle.
-  econstructor;intros.
-  - subst. econstructor. 2: unfold Basics.flip. all: eapply tagle'_PreOrder.
-  - inversion H. unfold tagle,Basics.flip in *.
-    eapply rev_rev_eq.
-    apply (partial_order_antisym tagle'_PartialOrder (rev x) (rev x0));eauto.
-  Qed.
- *)
+Lemma tagle_prefix_hd_le (n m : nat) (i j : Tag)
+      (H2 : m :: i ⊴ j)
+      (H1 : Prefix (n :: i) j)
+  : m <= n.
+Proof.
+  eapply prefix_eq in H1.
+  destructH.
+  subst. rewrite app_cons_assoc in H2. fold ([m] ++ i) in H2. eapply Tagle_app2 in H2.
+  fold (nil ++ [m]) in H2.
+  fold ([] :r: m) in H2.
+  eapply Tagle_le;eauto.
+Qed.
